WIP: asm proof

imp_compile/test.ml
@@ -13,14 +13,13 @@ open ImpMem1
 open ImpMem2
 open ImpLink
 
-(* Preprocessing Csharpminor programs *)
-(* ref: Velus, veluslib.ml *)
-(* let add_builtin p (name, (out, ins, b)) =
+
+
+(* let get_builtin (name, (out, ins, b)) =
  *   let env = Env.empty in
- *   let id = Camlcoq.intern_string name in
  *   let id' = Camlcoq.coqstring_of_camlstring name in
  *   let targs = List.map (C2C.convertTyp env) ins
- *                 |> Imp2Asm.ASMGEN.list_type_to_typelist in
+ *                 |> Imp2Asm.list_type_to_typelist in
  *   let tres = C2C.convertTyp env out in
  *   let sg = Ctypes.signature_of_type targs tres AST.cc_default in
  *   let ef =
@@ -31,42 +30,8 @@ open ImpLink
  *     && List.mem_assoc name C2C.builtins.builtin_functions
  *     then AST.EF_builtin(id', sg)
  *     else AST.EF_external(id', sg) in
- *   let decl = (id, AST.Gfun (AST.External ef)) in
- *   { p with AST.prog_defs = decl :: p.AST.prog_defs }
- * 
- * let add_builtins p =
- *   List.fold_left add_builtin p C2C.builtins_generic.builtin_functions *)
-
-
-(* let convert_builtin (name, (out, ins, b)) =
- *   let env = Env.empty in
- *   let id = Camlcoq.intern_string name in
- *   let id' = Camlcoq.coqstring_of_camlstring name in
- *   let targs = List.map (C2C.convertTyp env) ins
- *                 |> Imp2Asm.ASMGEN.list_type_to_typelist in
- *   let tres = C2C.convertTyp env out in
- *   let sg = Ctypes.signature_of_type targs tres AST.cc_default in
- *   let ef =
- *     if name = "malloc" then AST.EF_malloc else
- *     if name = "free" then AST.EF_free else
- *     if Str.string_match C2C.re_runtime name 0 then AST.EF_runtime(id', sg) else
- *     if Str.string_match C2C.re_builtin name 0
- *     && List.mem_assoc name C2C.builtins.builtin_functions
- *     then AST.EF_builtin(id', sg)
- *     else AST.EF_external(id', sg) in
- *   let decl = (id, AST.Gfun (AST.External ef)) in
+ *   let decl = (id', AST.Gfun (AST.External ef)) in
  *   decl *)
-
-(* let malloc_dec =
- *   ("malloc", (TPtr(TVoid [], []), [TPtr(TVoid [], [])], false))
- * 
- * let free_dec =
- *   ("free", (TVoid [], [TPtr(TVoid [], [])], false)) *)
-
-(* let app_builtins p =
- *   { p with AST.prog_defs = builtins @ p.AST.prog_defs } *)
-
-
 
 let get_builtin (name, (out, ins, b)) =
   let env = Env.empty in
@@ -83,40 +48,13 @@ let get_builtin (name, (out, ins, b)) =
     && List.mem_assoc name C2C.builtins.builtin_functions
     then AST.EF_builtin(id', sg)
     else AST.EF_external(id', sg) in
-  let decl = (id', AST.Gfun (AST.External ef)) in
+  let decl = (id', ef) in
   decl
 
 let builtins =
   List.map get_builtin C2C.builtins_generic.builtin_functions
 
 
-(* Csharpminor program compilation *)
-(* let compile_csm p ofile =
- *   let cl_built = app_builtins p in
- *   (\* Convert to Asm *\)
- *   (match Compiler.apply_partial
- *            (Imp2Asm.ASMGEN.transf_csharpminor_program cl_built)
- *            Asmexpand.expand_program with
- *    | Errors.OK asm ->
- *       (\* Print Asm in text form *\)
- *       let oc = open_out ofile in
- *       PrintAsm.print_program oc asm;
- *       close_out oc
- *    | Errors.Error msg ->
- *       let loc = file_loc ofile in
- *       fatal_error loc "%a"  print_error msg) *)
-
-
-(* (\* Imp program compilations *\)
- * let compile_imp p ofile =
- *   (\* Convert Imp to Csharpminor *\)
- *   let i2c = Imp2Csharpminor.compile_imp p in
- *   match i2c with
- *   | Errors.OK csm_out ->
- *      compile_csm csm_out ofile
- *   | Errors.Error msg ->
- *      let loc = file_loc ofile in
- *      fatal_error loc "%a"  print_error msg *)
 
 (* Imp program compilations *)
 let compile_imp p ofile =
